src/shared/logics/hlm/hlm.ts
@@ -1,7 +1,7 @@
 import * as Logic from '../logic';
+import * as Fmt from '../../format/format';
 import * as Ctx from '../../format/context';
 import * as FmtHLM from './meta';
-import { PlaceholderExpression } from '../generic/editHandler';
 import { HLMChecker } from './checker';
 import { HLMDisplay } from './display';
 
@@ -13,7 +13,7 @@ const hlmDefinitionTypes: Logic.LogicDefinitionTypeDescription[] = [
     createTypeExpression: () => new FmtHLM.MetaRefExpression_ExplicitOperator,
     createObjectContents: () => {
       let result = new FmtHLM.ObjectContents_ExplicitOperator;
-      result.definition = [new PlaceholderExpression(HLMExpressionType.ElementTerm)];
+      result.definition = [new Fmt.PlaceholderExpression(HLMExpressionType.ElementTerm)];
       return result;
     }
   },
@@ -24,7 +24,7 @@ const hlmDefinitionTypes: Logic.LogicDefinitionTypeDescription[] = [
     createTypeExpression: () => new FmtHLM.MetaRefExpression_SetOperator,
     createObjectContents: () => {
       let result = new FmtHLM.ObjectContents_SetOperator;
-      result.definition = [new PlaceholderExpression(HLMExpressionType.SetTerm)];
+      result.definition = [new Fmt.PlaceholderExpression(HLMExpressionType.SetTerm)];
       return result;
     }
   },
@@ -43,7 +43,7 @@ const hlmDefinitionTypes: Logic.LogicDefinitionTypeDescription[] = [
     createTypeExpression: () => new FmtHLM.MetaRefExpression_Predicate,
     createObjectContents: () => {
       let result = new FmtHLM.ObjectContents_Predicate;
-      result.definition = [new PlaceholderExpression(HLMExpressionType.Formula)];
+      result.definition = [new Fmt.PlaceholderExpression(HLMExpressionType.Formula)];
       return result;
     }
   },
@@ -55,7 +55,7 @@ const hlmDefinitionTypes: Logic.LogicDefinitionTypeDescription[] = [
     createTypeExpression: () => new FmtHLM.MetaRefExpression_StandardTheorem,
     createObjectContents: () => {
       let result = new FmtHLM.ObjectContents_StandardTheorem;
-      result.claim = new PlaceholderExpression(HLMExpressionType.Formula);
+      result.claim = new Fmt.PlaceholderExpression(HLMExpressionType.Formula);
       return result;
     }
   }
